src/cbor/pulse/CBOR.Pulse.API.Det.Rust.fst
@@ -1,0 +1,721 @@
+module CBOR.Pulse.API.Det.Rust
+open CBOR.Spec.Constants
+open CBOR.Pulse.API.Det
+open Pulse.Lib.Pervasives
+module Spec = CBOR.Spec.API.Format
+module Trade = Pulse.Lib.Trade.Util
+module U8 = FStar.UInt8
+module U64 = FStar.UInt64
+module S = Pulse.Lib.Slice
+module SZ = FStar.SizeT
+module Det = CBOR.Pulse.API.Det
+
+(* Validation, parsing and serialization *)
+
+type cbordet = cbor_det_t
+
+noextract [@@noextract_to "krml"]
+let cbor_det_parse_post
+  (input: S.slice U8.t)
+  (pm: perm)
+  (v: Seq.seq U8.t)
+  (res: option (cbordet & SZ.t))
+: Tot slprop
+= match res with
+  | None -> pts_to input #pm v ** pure (~ (exists v1 v2 . v == Spec.cbor_det_serialize v1 `Seq.append` v2))
+  | Some (res, len) ->
+    exists* v' .
+      cbor_det_match 1.0R res v' **
+      Trade.trade (cbor_det_match 1.0R res v') (pts_to input #pm v) ** pure (
+        SZ.v len <= Seq.length v /\
+        Seq.slice v 0 (SZ.v len) == Spec.cbor_det_serialize v'
+      )
+
+```pulse
+fn cbor_det_parse
+  (input: S.slice U8.t)
+  (#pm: perm)
+  (#v: Ghost.erased (Seq.seq U8.t))
+requires
+    (pts_to input #pm v)
+returns res: option (cbordet & SZ.t)
+ensures
+  cbor_det_parse_post input pm v res
+{
+  let len = cbor_det_validate input;
+  if (len = 0sz) {
+    fold (cbor_det_parse_post input pm v None);
+    None #(cbordet & SZ.t)
+  } else {
+    let res = Det.cbor_det_parse input len;
+    fold (cbor_det_parse_post input pm v (Some (res, len)));
+    Some (res, len)
+  }
+}
+```
+
+noextract [@@noextract_to "krml"]
+let cbor_det_size_postcond
+  (y: Spec.cbor)
+  (bound: SZ.t)
+  (res: option SZ.t)
+: Tot prop
+= let s = Spec.cbor_det_serialize y in
+  match res with
+  | None -> Seq.length s > SZ.v bound
+  | Some len -> Seq.length s == SZ.v len /\ SZ.v len <= SZ.v bound
+
+```pulse
+fn cbor_det_size
+  (x: cbordet)
+  (bound: SZ.t)
+  (#y: Ghost.erased Spec.cbor)
+  (#pm: perm)
+requires
+    (cbor_det_match pm x y)
+returns res: option SZ.t
+ensures
+  cbor_det_match pm x y **
+  pure (cbor_det_size_postcond y bound res)
+{
+  let size = Det.cbor_det_size x bound;
+  if (size = 0sz) {
+    None #SZ.t
+  } else {
+    Some size
+  }
+}
+```
+
+noextract [@@noextract_to "krml"]
+let cbor_det_serialize_postcond
+  (y: Spec.cbor)
+  (v: Seq.seq U8.t)
+  (v': Seq.seq U8.t)
+  (res: option SZ.t)
+: Tot prop
+= let s = Spec.cbor_det_serialize y in
+  match res with
+  | None -> Seq.length s > Seq.length v /\ v' == v
+  | Some len ->
+    Seq.length s == SZ.v len /\
+    SZ.v len <= Seq.length v /\
+    v' `Seq.equal` (s `Seq.append` Seq.slice v (SZ.v len) (Seq.length v))
+
+```pulse
+fn cbor_det_serialize
+  (x: cbordet)
+  (output: S.slice U8.t)
+  (#y: Ghost.erased Spec.cbor)
+  (#pm: perm)
+  (#v: Ghost.erased (Seq.seq U8.t))
+requires
+    (cbor_det_match pm x y ** pts_to output v)
+returns res: option SZ.t
+ensures
+    (exists* v' . cbor_det_match pm x y ** pts_to output v' ** pure (
+      cbor_det_serialize_postcond y v v' res
+    ))
+{
+  S.pts_to_len output;
+  let len = Det.cbor_det_size x (S.len output);
+  if (SZ.gt len 0sz) {
+    let Mktuple2 out rem = S.split output len;
+    S.pts_to_len out;
+    let len' = Det.cbor_det_serialize x out;
+    S.pts_to_len out;
+    S.join out rem output;
+    Some len'
+  } else {
+    None #SZ.t
+  }
+}
+```
+
+(* Constructors *)
+
+noextract [@@noextract_to "krml"]
+let cbor_det_mk_simple_value_post
+  (v: U8.t)
+  (res: option cbordet)
+: Tot slprop
+= match res with
+  | None -> emp
+  | Some res' -> exists* v' . cbor_det_match 1.0R res' v' ** pure (simple_value_wf v /\ v' == Spec.pack (Spec.CSimple v))
+
+```pulse
+fn cbor_det_mk_simple_value
+  (v: U8.t)
+requires emp
+returns res: option cbordet
+ensures
+  cbor_det_mk_simple_value_post v res **
+  pure (Some? res <==> simple_value_wf v)
+{
+  if simple_value_wf v {
+    let res = Det.cbor_det_mk_simple_value () v;
+    fold (cbor_det_mk_simple_value_post v (Some res));
+    Some res
+  }
+  else {
+    fold (cbor_det_mk_simple_value_post v None);
+    None #cbordet
+  }
+}
+```
+
+[@@no_auto_projectors]
+type cbor_det_int_kind =
+ | UInt64
+ | NegInt64
+
+```pulse
+fn cbor_det_mk_int64
+  (ty: cbor_det_int_kind)
+  (v: U64.t)
+requires emp
+returns res: cbordet
+ensures cbor_det_match 1.0R res (Spec.pack (Spec.CInt64 (if ty = UInt64 then cbor_major_type_uint64 else cbor_major_type_neg_int64) v))
+{
+  Det.cbor_det_mk_int64 () (if ty = UInt64 then cbor_major_type_uint64 else cbor_major_type_neg_int64) v
+}
+```
+
+[@@no_auto_projectors]
+type cbor_det_string_kind =
+| ByteString
+| TextString
+
+noextract [@@noextract_to "krml"]
+let cbor_det_mk_string_post
+  (ty: major_type_byte_string_or_text_string)
+  (s: S.slice U8.t)
+  (p: perm)
+  (v: Seq.seq U8.t)
+  (res: option cbordet)
+= match res with
+  | None -> pts_to s #p v
+  | Some res' -> exists* p' v' .
+    cbor_det_match p' res' (Spec.pack (Spec.CString ty v')) **
+    Trade.trade
+      (cbor_det_match p' res' (Spec.pack (Spec.CString ty v')))
+      (pts_to s #p v) **
+    pure (v' == v)
+
+let uint64_max_prop : squash (pow2 64 - 1 == 18446744073709551615) =
+  assert_norm (pow2 64 - 1 == 18446744073709551615)
+
+```pulse
+fn cbor_det_mk_string
+  (ty: cbor_det_string_kind)
+  (s: S.slice U8.t)
+  (#p: perm)
+  (#v: Ghost.erased (Seq.seq U8.t))
+requires pts_to s #p v
+returns res: option cbordet
+ensures
+  cbor_det_mk_string_post (if ty = ByteString then cbor_major_type_byte_string else cbor_major_type_text_string) s p v res **
+  pure (Some? res <==> FStar.UInt.fits (SZ.v (S.len s)) U64.n)
+{
+  let sq: squash (SZ.fits_u64) = assume (SZ.fits_u64);
+  S.pts_to_len s;
+  if SZ.gt (S.len s) (SZ.uint64_to_sizet 18446744073709551615uL) {
+    fold (cbor_det_mk_string_post (if ty = ByteString then cbor_major_type_byte_string else cbor_major_type_text_string) s p v None);
+    None #cbordet
+  } else {
+    let res = Det.cbor_det_mk_string () (if ty = ByteString then cbor_major_type_byte_string else cbor_major_type_text_string) s;
+    fold (cbor_det_mk_string_post (if ty = ByteString then cbor_major_type_byte_string else cbor_major_type_text_string) s p v (Some res));
+    Some res
+  }
+}
+```
+
+let cbor_det_mk_tagged tag r #pr #v #pv #v' = Det.cbor_det_mk_tagged () tag r #pr #v #pv #v'
+
+let cbor_det_mk_map_entry xk xv #pk #vk #pv #vv = Det.cbor_det_mk_map_entry () xk xv #pk #vk #pv #vv
+
+module PM = Pulse.Lib.SeqMatch
+
+noextract [@@noextract_to "krml"]
+let cbor_det_mk_array_post
+  (a: S.slice cbordet)
+  (pa: perm)
+  (va: (Seq.seq cbordet))
+  (pv: perm)
+  (vv: (list Spec.cbor))
+  (res: option cbordet)
+: Tot slprop
+= match res with
+  | None ->
+    pts_to a #pa va **
+    PM.seq_list_match va vv (cbor_det_match pv)
+  | Some res ->
+    exists* p' v' .
+      cbor_det_match p' res (Spec.pack (Spec.CArray v')) **
+      Trade.trade
+        (cbor_det_match p' res (Spec.pack (Spec.CArray v')))
+        (pts_to a #pa va **
+          PM.seq_list_match va vv (cbor_det_match pv)
+        ) **
+        pure (
+          v' == vv
+        )
+
+```pulse
+fn cbor_det_mk_array
+  (a: S.slice cbordet)
+  (#pa: perm)
+  (#va: Ghost.erased (Seq.seq cbordet))
+  (#pv: perm)
+  (#vv: Ghost.erased (list Spec.cbor))
+requires
+    pts_to a #pa va **
+    PM.seq_list_match va vv (cbor_det_match pv)
+returns res: option cbordet
+ensures
+  cbor_det_mk_array_post a pa va pv vv res **
+  pure (Some? res <==> FStar.UInt.fits (SZ.v (S.len a)) U64.n)
+{
+  let _ : squash SZ.fits_u64 = assume (SZ.fits_u64);
+  if SZ.gt (S.len a) (SZ.uint64_to_sizet 18446744073709551615uL) {
+    fold (cbor_det_mk_array_post a pa va pv vv None);
+    None #cbordet;
+  } else {
+    let res = Det.cbor_det_mk_array () a;
+    fold (cbor_det_mk_array_post a pa va pv vv (Some res));
+    Some res
+  }
+}
+```
+
+let cbor_det_mk_map a #va #pv #vv = Det.cbor_det_mk_map_gen () a #va #pv #vv
+
+(* Destructors *)
+
+let cbor_det_equal x1 x2 #p1 #p2 #v1 #v2 = Det.cbor_det_equal () x1 x2 #p1 #p2 #v1 #v2
+
+noextract [@@noextract_to "krml"]
+let cbor_det_tagged_match (p: perm) (tag: U64.t) (payload: cbor_det_t) (v: Spec.cbor) : Tot slprop =
+  exists* v' .
+    cbor_det_match p payload v' **
+    pure (Spec.unpack v == Spec.CTagged tag v')
+
+[@@CAbstractStruct; no_auto_projectors]
+noeq
+type cbor_det_array = {
+  array: (array: cbordet { CaseArray? (cbor_det_case array) }) ;
+}
+
+noextract [@@noextract_to "krml"]
+let cbor_det_array_match (p: perm) (a: cbor_det_array) (v: Spec.cbor) : Tot slprop =
+  cbor_det_match p a.array v **
+  pure (Spec.CArray? (Spec.unpack v))
+
+[@@CAbstractStruct; no_auto_projectors]
+noeq
+type cbor_det_map = {
+  map: (map: cbordet { CaseMap? (cbor_det_case map) });
+}
+
+noextract [@@noextract_to "krml"]
+let cbor_det_map_match (p: perm) (a: cbor_det_map) (v: Spec.cbor) : Tot slprop =
+  cbor_det_match p a.map v **
+  pure (Spec.CMap? (Spec.unpack v))
+
+noextract [@@noextract_to "krml"]
+let cbor_det_string_match (t: major_type_byte_string_or_text_string) (p: perm) (a: S.slice U8.t) (v: Spec.cbor) : Tot slprop =
+  exists* (v': Seq.seq U8.t) .
+    pts_to a #p v' **
+    pure (Spec.CString? (Spec.unpack v) /\ v' == Spec.CString?.v (Spec.unpack v) /\ t == Spec.CString?.typ (Spec.unpack v))
+
+noeq [@@no_auto_projectors]
+type cbor_det_view =
+| Int64: (kind: cbor_det_int_kind) -> (value: U64.t) -> cbor_det_view
+| String: (kind: cbor_det_string_kind) -> (payload: S.slice U8.t) -> cbor_det_view
+| Array of cbor_det_array
+| Map of cbor_det_map
+| Tagged: (tag: U64.t) -> (payload: cbor_det_t) -> cbor_det_view
+| SimpleValue of simple_value
+
+noextract [@@noextract_to "krml"]
+let cbor_det_view_match
+  (p: perm)
+  (x: cbor_det_view)
+  (v: Spec.cbor)
+: Tot slprop
+= match x with
+  | Int64 k i -> pure (v == Spec.pack (Spec.CInt64 (if UInt64? k then cbor_major_type_uint64 else cbor_major_type_neg_int64) i))
+  | String k s -> cbor_det_string_match (if ByteString? k then cbor_major_type_byte_string else cbor_major_type_text_string)  p s v
+  | Tagged tag pl -> cbor_det_tagged_match p tag pl v
+  | Array a -> cbor_det_array_match p a v
+  | Map m -> cbor_det_map_match p m v
+  | SimpleValue i -> pure (v == Spec.pack (Spec.CSimple i))
+
+```pulse
+fn cbor_det_destruct
+  (c: cbordet)
+  (#p: perm)
+  (#v: Ghost.erased Spec.cbor)
+requires
+  cbor_det_match p c v
+returns w: cbor_det_view
+ensures exists* p' .
+  cbor_det_view_match p' w v **
+  Trade.trade
+    (cbor_det_view_match p' w v)
+    (cbor_det_match p c v)
+{
+  let ty = cbor_det_major_type () c;
+  cbor_det_case_correct c;
+  if (ty = cbor_major_type_uint64 || ty = cbor_major_type_neg_int64) {
+    let k = (if ty = cbor_major_type_uint64 then UInt64 else NegInt64);
+    let i = cbor_det_read_uint64 () c;
+    fold (cbor_det_view_match p (Int64 k i) v);
+    ghost fn aux (_: unit)
+      requires cbor_det_match p c v ** cbor_det_view_match p (Int64 k i) v
+      ensures cbor_det_match p c v
+    {
+      unfold (cbor_det_view_match p (Int64 k i) v)
+    };
+    Trade.intro _ _ _ aux;
+    Int64 k i
+  }
+  else if (ty = cbor_major_type_byte_string || ty = cbor_major_type_text_string) {
+    let k = (if ty = cbor_major_type_byte_string then ByteString else TextString);
+    let s = cbor_det_get_string () c;
+    with p' v' . assert (pts_to s #p' v');
+    fold (cbor_det_string_match ty p' s v);
+    fold (cbor_det_view_match p' (String k s) v);
+    ghost fn aux (_: unit)
+    requires emp ** cbor_det_view_match p' (String k s) v
+    ensures pts_to s #p' v'
+    {
+      unfold (cbor_det_view_match p' (String k s) v);
+      unfold (cbor_det_string_match ty p' s v);
+    };
+    Trade.intro _ _ _ aux;
+    Trade.trans _ _ (cbor_det_match p c v);
+    String k s
+  }
+  else if (ty = cbor_major_type_array) {
+    let res : cbor_det_array = { array = c };
+    fold (cbor_det_array_match p res v);
+    fold (cbor_det_view_match p (Array res) v);
+    ghost fn aux (_: unit)
+    requires emp ** cbor_det_view_match p (Array res) v
+    ensures cbor_det_match p c v
+    {
+      unfold (cbor_det_view_match p (Array res) v);
+      unfold (cbor_det_array_match p res v);
+    };
+    Trade.intro _ _ _ aux;
+    Array res
+  }
+  else if (ty = cbor_major_type_map) {
+    let res : cbor_det_map = { map = c };
+    fold (cbor_det_map_match p res v);
+    fold (cbor_det_view_match p (Map res) v);
+    ghost fn aux (_: unit)
+    requires emp ** cbor_det_view_match p (Map res) v
+    ensures cbor_det_match p c v
+    {
+      unfold (cbor_det_view_match p (Map res) v);
+      unfold (cbor_det_map_match p res v);
+    };
+    Trade.intro _ _ _ aux;
+    Map res
+  }
+  else if (ty = cbor_major_type_tagged) {
+    let tag = cbor_det_get_tagged_tag () c;
+    let payload = cbor_det_get_tagged_payload () c;
+    with p' v' . assert (cbor_det_match p' payload v');
+    fold (cbor_det_tagged_match p' tag payload v);
+    fold (cbor_det_view_match p' (Tagged tag payload) v);
+    ghost fn aux (_: unit)
+    requires emp ** cbor_det_view_match p' (Tagged tag payload) v
+    ensures cbor_det_match p' payload v'
+    {
+      unfold (cbor_det_view_match p' (Tagged tag payload) v);
+      unfold (cbor_det_tagged_match p' tag payload v);
+    };
+    Trade.intro _ _ _ aux;
+    Trade.trans _ _ (cbor_det_match p c v);
+    Tagged tag payload
+  }
+  else {
+    let i = cbor_det_read_simple_value () c;
+    fold (cbor_det_view_match p (SimpleValue i) v);
+    ghost fn aux (_: unit)
+      requires cbor_det_match p c v ** cbor_det_view_match p (SimpleValue i) v
+      ensures cbor_det_match p c v
+    {
+      unfold (cbor_det_view_match p (SimpleValue i) v)
+    };
+    Trade.intro _ _ _ aux;
+    SimpleValue i
+  }
+}
+```
+
+```pulse
+fn cbor_det_get_array_length
+  (x: cbor_det_array)
+  (#p: perm)
+  (#y: Ghost.erased Spec.cbor)
+requires
+  cbor_det_array_match p x y
+returns res: U64.t
+ensures
+  cbor_det_array_match p x y ** pure (
+    get_array_length_post y res
+  )
+{
+  unfold (cbor_det_array_match p x y);
+  let res = Det.cbor_det_get_array_length () x.array;
+  fold (cbor_det_array_match p x y);
+  res
+}
+```
+
+```pulse
+ghost
+fn cbor_det_array_match_elim
+  (x: cbor_det_array)
+  (#p: perm)
+  (#y: Spec.cbor)
+requires cbor_det_array_match p x y
+ensures cbor_det_match p x.array y **
+  Trade.trade (cbor_det_match p x.array y) (cbor_det_array_match p x y) **
+  pure (Spec.CArray? (Spec.unpack y))
+{
+  unfold (cbor_det_array_match p x y);
+  ghost fn aux (_: unit)
+  requires emp ** cbor_det_match p x.array y
+  ensures cbor_det_array_match p x y
+  {
+    fold (cbor_det_array_match p x y);
+  };
+  Trade.intro _ _ _ aux;
+}
+```
+
+```pulse
+fn cbor_det_array_iterator_start
+  (x: cbor_det_array)
+  (#p: perm)
+  (#y: Ghost.erased Spec.cbor)
+requires
+  (cbor_det_array_match p x y)
+returns res: cbor_det_array_iterator_t
+ensures
+    (exists* p' l' .
+      cbor_det_array_iterator_match p' res l' **
+      Trade.trade
+        (cbor_det_array_iterator_match p' res l')
+        (cbor_det_array_match p x y) **
+      pure (
+        Spec.CArray? (Spec.unpack y) /\
+        l' == Spec.CArray?.v (Spec.unpack y)
+    ))
+{
+  cbor_det_array_match_elim x;
+  let res = Det.cbor_det_array_iterator_start () x.array;
+  Trade.trans _ _ (cbor_det_array_match p x y);
+  res
+}
+```
+
+let cbor_det_array_iterator_is_empty x #p #y = Det.cbor_det_array_iterator_is_empty () x #p #y
+
+let cbor_det_array_iterator_next x #y #py #z = Det.cbor_det_array_iterator_next () x #y #py #z
+
+noextract [@@noextract_to "krml"]
+let safe_get_array_item_post
+  (x: cbor_det_array)
+  (i: U64.t)
+  (p: perm)
+  (y: Spec.cbor)
+  (res: option cbordet)
+: Tot slprop
+= match res with
+  | None -> cbor_det_array_match p x y ** pure (Spec.CArray? (Spec.unpack y) /\ U64.v i >= List.Tot.length (Spec.CArray?.v (Spec.unpack y)))
+  | Some res' -> exists* p' y' .
+    cbor_det_match p' res' y' **
+    Trade.trade (cbor_det_match p' res' y') (cbor_det_array_match p x y) **
+    pure (get_array_item_post i y y')
+
+```pulse
+fn cbor_det_get_array_item
+  (x: cbor_det_array)
+  (i: U64.t)
+  (#p: perm)
+  (#y: Ghost.erased Spec.cbor)
+requires
+  cbor_det_array_match p x y
+returns res: option cbordet
+ensures
+  safe_get_array_item_post x i p y res
+{
+  let len = cbor_det_get_array_length x;
+  if U64.gte i len {
+    fold (safe_get_array_item_post x i p y None);
+    None #cbordet
+  } else {
+    cbor_det_array_match_elim x;
+    let res = Det.cbor_det_get_array_item () x.array i;
+    Trade.trans _ _ (cbor_det_array_match p x y);
+    fold (safe_get_array_item_post x i p y (Some res));
+    Some res
+  }
+}
+```
+
+```pulse
+fn cbor_det_map_length
+  (x: cbor_det_map)
+  (#p: perm)
+  (#y: Ghost.erased Spec.cbor)
+requires
+  cbor_det_map_match p x y
+returns res: U64.t
+ensures
+  cbor_det_map_match p x y ** pure (
+    get_map_length_post y res
+  )
+{
+  unfold (cbor_det_map_match p x y);
+  let res = Det.cbor_det_get_map_length () x.map;
+  fold (cbor_det_map_match p x y);
+  res
+}
+```
+
+```pulse
+ghost
+fn cbor_det_map_match_elim
+  (x: cbor_det_map)
+  (#p: perm)
+  (#y: Spec.cbor)
+requires cbor_det_map_match p x y
+ensures cbor_det_match p x.map y **
+  Trade.trade (cbor_det_match p x.map y) (cbor_det_map_match p x y) **
+  pure (Spec.CMap? (Spec.unpack y))
+{
+  unfold (cbor_det_map_match p x y);
+  ghost fn aux (_: unit)
+  requires emp ** cbor_det_match p x.map y
+  ensures cbor_det_map_match p x y
+  {
+    fold (cbor_det_map_match p x y);
+  };
+  Trade.intro _ _ _ aux;
+}
+```
+
+```pulse
+fn cbor_det_map_iterator_start
+  (x: cbor_det_map)
+  (#p: perm)
+  (#y: Ghost.erased Spec.cbor)
+requires
+  (cbor_det_map_match p x y)
+returns res: cbor_det_map_iterator_t
+ensures
+    (exists* p' l' .
+      cbor_det_map_iterator_match p' res l' **
+      Trade.trade
+        (cbor_det_map_iterator_match p' res l')
+        (cbor_det_map_match p x y) **
+      pure (
+        map_iterator_start_post y l'
+    ))
+{
+  cbor_det_map_match_elim x;
+  let res = Det.cbor_det_map_iterator_start () x.map;
+  Trade.trans _ _ (cbor_det_map_match p x y);
+  res
+}
+```
+
+let cbor_det_map_iterator_is_empty x #p #y = Det.cbor_det_map_iterator_is_empty () x #p #y
+
+let cbor_det_map_iterator_next x #y #py #z = Det.cbor_det_map_iterator_next () x #y #py #z
+
+let cbor_det_map_entry_key x2 #p #v2 = Det.cbor_det_map_entry_key () x2 #p #v2
+
+let cbor_det_map_entry_value x2 #p #v2 = Det.cbor_det_map_entry_value () x2 #p #v2
+
+noextract [@@noextract_to "krml"]
+let safe_map_get_post
+  (x: cbor_det_map)
+  (px: perm)
+  (vx: Spec.cbor)
+  (vk: Spec.cbor)
+  (res: option cbordet)
+: Tot slprop
+= match res with
+  | None ->
+    cbor_det_map_match px x vx ** pure (Spec.CMap? (Spec.unpack vx) /\ None? (Spec.cbor_map_get (Spec.CMap?.c (Spec.unpack vx)) vk))
+  | Some x' ->
+    exists* px' vx' .
+      cbor_det_match px' x' vx' **
+      Trade.trade
+        (cbor_det_match px' x' vx')
+        (cbor_det_map_match px x vx) **
+      pure (Spec.CMap? (Spec.unpack vx) /\ Spec.cbor_map_get (Spec.CMap?.c (Spec.unpack vx)) vk == Some vx')  
+
+```pulse
+ghost
+fn cbor_det_map_get_post_to_safe
+  (x: cbor_det_map)
+  (px: perm)
+  (vx: Spec.cbor)
+  (vk: Spec.cbor)
+  (res: option cbordet)
+requires
+  map_get_post cbor_det_match x.map px vx vk res **
+  Trade.trade (cbor_det_match px x.map vx) (cbor_det_map_match px x vx)
+ensures
+  safe_map_get_post x px vx vk res
+{
+  match res {
+    None -> {
+      unfold (map_get_post cbor_det_match x.map px vx vk None);
+      unfold (map_get_post_none cbor_det_match x.map px vx vk);
+      Trade.elim _ _;
+      fold (safe_map_get_post x px vx vk None);
+    }
+    Some res' -> {
+      unfold (map_get_post cbor_det_match x.map px vx vk (Some res'));
+      unfold (map_get_post_some cbor_det_match x.map px vx vk res');
+      Trade.trans _ _ (cbor_det_map_match px x vx);
+      fold (safe_map_get_post x px vx vk (Some res'));
+    }
+  }
+}
+```
+
+```pulse
+fn cbor_det_map_get
+  (x: cbor_det_map)
+  (k: cbordet)
+  (#px: perm)
+  (#vx: Ghost.erased Spec.cbor)
+  (#pk: perm)
+  (#vk: Ghost.erased Spec.cbor)
+requires
+    (cbor_det_map_match px x vx ** cbor_det_match pk k vk)
+returns res: option cbordet
+ensures
+    (
+      cbor_det_match pk k vk **
+      safe_map_get_post x px vx vk res **
+      pure (Spec.CMap? (Spec.unpack vx) /\ (Some? (Spec.cbor_map_get (Spec.CMap?.c (Spec.unpack vx)) vk) == Some? res))
+    )
+{
+  cbor_det_map_match_elim x;
+  let res = Det.cbor_det_map_get () x.map k;
+  cbor_det_map_get_post_to_safe x px vx vk res;
+  res
+}
+```
